more edits

rocq/stlc/red.v
@@ -12,7 +12,7 @@ Import ScopedNotations.
 
 Definition is_value {n} (e : Tm n) : bool := 
   match e with 
-  | var_Tm _ => true  (* is this ok? why or why not? *)
+  | var _ => true  (* is this ok? why or why not? *)
   | abs _ => true
   | lit k => true
   | _ => false
@@ -26,7 +26,7 @@ Inductive step : Tm 0 -> Tm 0 -> Prop :=
 
  | s_beta e v : 
     is_value v = true ->
-    step (app (abs e) v) (e [v .: null])
+    step (app (abs e) v) (e [v..])
 
  | s_app_cong1 e1 e1' e2 : 
     step e1 e1' ->
@@ -36,8 +36,6 @@ Inductive step : Tm 0 -> Tm 0 -> Prop :=
     is_value v = true ->
     step e2 e2' ->
     step (app v e2) (app v e2')
-
-
 .
 
 End Small.
@@ -54,10 +52,8 @@ Inductive step : Tm 0 -> Tm 0 -> Prop :=
   | s_app  e1 e1' e2 v1 v2 :
     step e1 (abs e1') ->
     step e2 v1 ->
-    step (e1' [v1 .: null ]) v2 ->
+    step (e1' [v1 .. ]) v2 ->
     step (app e1 e2) v2
-
-
 .
 
 
@@ -79,7 +75,7 @@ Definition Env n := fin n -> Val.
 Inductive step {n} (ρ : Env n) : Tm n -> Val -> Prop := 
 
   | s_var x : 
-    step ρ (var_Tm x) (ρ x)
+    step ρ (var x) (ρ x)
 
   | s_abs e : 
     step ρ (abs e) (v_clo ρ e)
@@ -90,14 +86,20 @@ Inductive step {n} (ρ : Env n) : Tm n -> Val -> Prop :=
     step (v1 .: ρ') e1' v2 ->
     step ρ (app e1 e2) v2
 
+  | s_lit k : 
+    step ρ (lit k) (v_lit k)
+
 
 .
 
 
 End BigEnv.   
 
-Module RedNotations.
-Infix "⟼" := Small.step (at level 70).
+Module RedNotations.  
+Infix "⤳"  := Small.step (at level 70).
+Infix "⤳*" := (multi Small.step) (at level 70).
+Notation "e ⟱ v" := 
+  (e ⤳* v /\ is_value (v : Tm 0) = true) (at level 70).
 Infix "⇓"   := Big.step   (at level 70).
-Coercion BigEnv.v_lit : nat >-> BigEnv.Val.
+Notation "< ρ | e > ⇓ v" := (BigEnv.step ρ e v) (at level 70).
 End RedNotations.
