rocq/stlc/typing.v
@@ -1,15 +1,23 @@
 From Stdlib Require Export ssreflect.
 From Stdlib Require Export Program.Equality.
 Require Export common.fintype.
+Require Export common.core.
+
 Require Export stlc.syntax.
 
 Import ScopedNotations.
+
+Module SyntaxNotations.
+Notation "⇑ σ" := (var var_zero .: σ >> ren_Tm ↑) (at level 70) : subst_scope.
+End SyntaxNotations.
+
+Import SyntaxNotations.
 
 Definition Ctx (n : nat) := fin n -> Ty.
 
 Inductive typing {n} (Γ : Ctx n) : Tm n -> Ty -> Prop := 
   | t_var x : 
-    typing Γ (var_Tm x) (Γ x)
+    typing Γ (var x) (Γ x)
 
   | t_abs e τ1 τ2 : 
     typing (τ1 .: Γ) e τ2 -> 
@@ -23,10 +31,16 @@ Inductive typing {n} (Γ : Ctx n) : Tm n -> Ty -> Prop :=
   | t_lit k : 
     typing Γ (lit k) Nat
 
-
 .
 
 Module TypingNotations.
 Export ScopedNotations.
-Notation "Γ |- e :: τ" := (typing Γ e τ) (at level 70).
+Export SyntaxNotations.
+Notation "Γ |- e ∈ τ" := (typing Γ e τ) (at level 70).
 End TypingNotations.
+
+Import TypingNotations.
+
+
+
+
